small steps and rewrite idea for WorldPath etc

Pdl/Paths.lean
@@ -1,26 +1,30 @@
 
 import Pdl.Unfold
 
-def atomRel (M : KripkeModel W) (v w : W) := ∃ a, relate M (·a) v w
+def atomRel {W} (M : KripkeModel W) (v w : W) := ∃ a, relate M (·a) v w
 
-def WorldPath {W} (M : KripkeModel W) := Subtype $ List.Chain' (atomRel M)
+abbrev WorldPath {W} (M : KripkeModel W) := Subtype $ List.Chain' (atomRel M)
 
-/-- Does path `π` witness `¬□(δ,ξ)` at `v0`? -/
+@[simp]
+def WorldPath.tail (π : WorldPath M) : WorldPath M := ⟨π.1.tail, π.2.tail⟩
+
+/-- Does path `π` starting at v0 witness `¬□(δ,ξ)`? -/
+-- IDEA: rewrite this as an inductive prop instead of matching?
 def witnessing (M : KripkeModel W) (v0 : W) (π : WorldPath M) (δ : List Program) (ξ : Formula) : Prop :=
-  match π, δ with
+  match π.1, δ with
     -- Case |π| = 0:
-    | ⟨[],_⟩, [] => (M,v0) ⊨ (~ξ)
-    | ⟨[],_⟩, (_::_) => False
+    | [], [] => (M,v0) ⊨ (~ξ)
+    | [], _::_ => False
     -- Case |π| > 0:
-    | ⟨_::_, _⟩ , [] => False
-    | π@⟨v1::rest, _⟩ , α::γs =>
-        (∃ a, α = (Program.atom_prog a) ∧ witnessing M v1 ⟨rest, sorry⟩ γs ξ)
+    | _ :: _ , [] => False
+    | v1 :: rest , α::γs =>
+        (∃ a, α = (Program.atom_prog a) ∧ witnessing M v1 π.tail γs ξ)
       ∨ ∃ Fβ ∈ H α,
         (M,v0) ⊨ Fβ.1
         ∧ (
           (Fβ.2 = ε ∧ witnessing M v0 π γs ξ)
           ∨
-          (∃ a, ∃ ηs, Fβ.2 = ((Program.atom_prog a) :: ηs) ∧ witnessing M v1 ⟨rest, sorry⟩ (ηs ++ γs) ξ)
+          (∃ a, ∃ ηs, Fβ.2 = ((Program.atom_prog a) :: ηs) ∧ witnessing M v1 π.tail (ηs ++ γs) ξ)
           )
 termination_by (π.1.length, δ.length)
 decreasing_by
@@ -33,23 +37,44 @@ theorem existsWitnessPath {M : KripkeModel W} δ v :
     simp [modelCanSemImplyForm, witnessing]
     constructor
     · intro nvXi
-      use ⟨[], by simp⟩
+      use [], (by simp)
       simp only [witnessing, modelCanSemImplyForm, evaluatePoint, evaluate]
       exact nvXi
-    · rintro ⟨π, foo⟩
-      rcases π with ⟨no|bla, foo⟩
-      · simp [witnessing, modelCanSemImplyForm, evaluatePoint, evaluate] at *
-        assumption
-      · simp [witnessing] at *
+    · rintro ⟨π, ⟨l, foo⟩⟩
+      cases π
+      · simp_all [witnessing, modelCanSemImplyForm]
+      · exfalso; unfold witnessing at foo; tauto
   case cons d δ IH =>
     simp only [Formula.boxes]
     constructor
     · simp only [modelCanSemImplyForm, evaluatePoint, evaluate, not_forall, exists_prop, forall_exists_index, and_imp] at *
       intro w v_d_w not_w_
       rw [IH] at not_w_
-      -- rcases not_w_ with ⟨π, wit⟩
+      clear IH
+      rcases not_w_ with ⟨⟨π, l⟩, wit⟩
       -- simp [witnessing] at *
-
-      sorry
+      cases d
+      all_goals simp only [relate] at v_d_w
+      case atom_prog a =>
+        cases π <;> cases δ -- yield four cases, matching those in `def witnessing`.
+        · refine ⟨⟨[w], ?_⟩, ?_⟩
+          simp
+          unfold witnessing
+          simp
+          left
+          assumption
+        · exfalso; simp [witnessing] at wit
+        · exfalso; unfold witnessing at wit; exact wit
+        · unfold witnessing
+          simp
+          sorry
+      case test φ =>
+        sorry
+      case sequence α β =>
+        sorry
+      case union α β =>
+        sorry
+      case star α =>
+        sorry
     ·
       sorry
